sync

proof/iu_system/decl/def_extra.v
@@ -90,8 +90,8 @@ Inductive d_sub : denv -> dtyp -> dtyp -> Prop :=    (* defn d_sub *)
      d_sub E (dtyp_all S1) (dtyp_all T1)
  | d_sub_alll : forall (L:vars) (E:denv) (S1 T1 T2:dtyp),
      dneq_all T1 ->
-     (* dneq_intersection T1 -> *)
-     (* dneq_union T1 ->  *)
+     dneq_intersection T1 ->
+     dneq_union T1 -> 
      ( forall X , X \notin L -> ds_in X  (open_dtyp_wrt_dtyp  S1   (dtyp_var_f X) ) ) ->
      dwf_typ E T2 ->
      dmono_typ T2 ->
@@ -122,7 +122,37 @@ Inductive d_sub : denv -> dtyp -> dtyp -> Prop :=    (* defn d_sub *)
      d_sub E S2 T1 ->
      d_sub E (dtyp_union S1 S2) T1.
 
-Inductive d_typing_mode :=
+Inductive d_inftapp : denv -> dtyp -> dtyp -> dtyp -> Prop := 
+| d_inftapp_bot : forall (E:denv) (T1:dtyp),
+    dwf_typ E T1 ->
+    d_inftapp E dtyp_bot T1 dtyp_bot
+| d_inftapp_all : forall (E:denv) (T1 T2:dtyp),
+    dwf_typ E (dtyp_all T1) ->
+    dwf_typ E T2 ->
+    d_inftapp E (dtyp_all T1) T2 (open_dtyp_wrt_dtyp  T1   T2 ).
+
+Inductive d_infabs : denv -> dtyp -> dtyp -> Prop := 
+| d_infabs_bot : forall (E:denv),
+    d_infabs E dtyp_bot (dtyp_arrow dtyp_top dtyp_bot)
+| d_infabs_arr : forall (E:denv) (T1 T2:dtyp),
+    d_infabs E (dtyp_arrow T1 T2) (dtyp_arrow T1 T2)
+| d_infabs_all : forall (E:denv) (T1 T2 T3:dtyp),
+    dmono_typ T2 -> 
+    dwf_typ E T2 ->
+    dwf_typ E (dtyp_all T1) ->
+    d_infabs E  (open_dtyp_wrt_dtyp  T1   T2 ) T3 ->
+    d_infabs E (dtyp_all T1) T3
+| d_infabs_intersection1 : forall (E:denv) (T1 T2 T3:dtyp),
+    dwf_typ E T2 ->
+    d_infabs E T1 T3 ->
+    d_infabs E (dtyp_intersection T1 T2) T3
+| d_infabs_intersection2 : forall (E:denv) (T1 T2 T3:dtyp),
+    dwf_typ E T1 ->
+    d_infabs E T2 T3 ->
+    d_infabs E (dtyp_intersection T1 T2) T3
+.
+
+(* Inductive d_typing_mode :=
     | d_typingmode_inf 
     | d_typingmode_chk
     | d_typingmode_infapp (T1 : dtyp).
@@ -214,4 +244,77 @@ dwf_typ E (dtyp_all T1) ->
     d_typing E e ( d_typingmode_infapp (dtyp_union S1 S2) ) T1
     .
 
+ *)
 
+(* Inductive d_env_sub : denv -> denv -> Prop :=
+| d_envsub_nil : d_env_sub nil nil
+| d_envsub_tvar : forall (E1 E2:denv) (X:typvar) (T1 T2:dtyp),
+    d_env_sub E1 E2 ->
+    d_env_sub ( ( X ~ dbind_tvar_empty ) ++ E1 ) ( ( X ~ dbind_tvar_empty ) ++ E2 )
+| d_envsub_stvar : forall (E1 E2:denv) (SX:stypvar) (T1 T2:dtyp),
+    d_env_sub E1 E2 ->
+    d_env_sub ( ( SX ~ dbind_stvar_empty ) ++ E1 ) ( ( SX ~ dbind_stvar_empty ) ++ E2 )
+| d_envsub_var : forall (E1 E2:denv) (x:expvar) (T1 T2:dtyp),
+    d_env_sub E1 E2 ->
+    d_sub E2 T1 T2 ->
+    d_env_sub ( ( x ~ dbind_typ T1 ) ++ E1 ) ( ( x ~ dbind_typ T2 ) ++ E2 )
+. *)
+
+Inductive d_typing_mode :=
+| d_typingmode_inf 
+| d_typingmode_chk.
+
+Inductive d_typing : denv -> dexp -> d_typing_mode -> dtyp -> Prop :=
+| d_typing_infvar : forall (E:denv) (x:expvar) (T1:dtyp),
+    dwf_env E ->
+    binds ( x )  ( (dbind_typ T1) ) ( E )  ->
+    d_typing E (dexp_var_f x) d_typingmode_inf T1
+| d_typing_infanno : forall (E:denv) (e:dexp) (T1:dtyp),
+    dwf_typ E T1 ->
+    d_typing E e d_typingmode_chk T1 ->
+    d_typing E  ( (dexp_anno e T1) )  d_typingmode_inf T1
+| d_typinginf_unit : forall (E:denv),
+    dwf_env E ->
+    d_typing E dexp_unit d_typingmode_inf dtyp_unit
+| d_typing_infapp : forall (E:denv) (e1 e2:dexp) (T1 T2 T3:dtyp),
+    d_typing E e1 d_typingmode_inf T1 ->
+    d_infabs E T1 (dtyp_arrow T2 T3) ->
+    d_typing E e2 d_typingmode_chk T2 ->
+    d_typing E  ( (dexp_app e1 e2) ) d_typingmode_inf T3
+| d_typing_inftabs : forall (L:vars) (E:denv) (e:dexp) (T1:dtyp),
+dwf_typ E (dtyp_all T1) ->
+    ( forall X , X \notin  L  -> d_typing  ( X ~ dbind_tvar_empty  ++  E ) (dexp_anno  ( open_dexp_wrt_dtyp e (dtyp_var_f X) )  ( open_dtyp_wrt_dtyp T1 (dtyp_var_f X) ) ) d_typingmode_chk ( open_dtyp_wrt_dtyp T1 (dtyp_var_f X) )  )  ->
+    d_typing E (dexp_tabs (dbody_anno e T1)) d_typingmode_inf (dtyp_all T1)
+| d_typing_inftapp : forall (E:denv) (e1:dexp) (T1 T2 T3:dtyp),
+    dwf_typ E T2 ->
+    d_typing E e1 d_typingmode_inf T1 ->
+    d_inftapp E T1 T2 T3 ->
+    d_typing E (dexp_tapp e1 T2) d_typingmode_inf T3
+| d_typing_chkabstop : forall (L:vars) (E:denv) (e:dexp),
+    ( forall x , x \notin  L  -> d_typing  ( x ~ (dbind_typ dtyp_bot)  ++  E )   ( open_dexp_wrt_dexp e (dexp_var_f x) ) d_typingmode_chk dtyp_top )  ->
+    d_typing E (dexp_abs e) d_typingmode_chk dtyp_top
+| d_typing_chkabs : forall (L:vars) (E:denv) (e:dexp) (T1 T2:dtyp),
+    dwf_typ E T1 ->
+    ( forall x , x \notin  L  -> d_typing  ( x ~ (dbind_typ T1)  ++  E )  ( open_dexp_wrt_dexp e (dexp_var_f x) ) d_typingmode_chk T2 )  ->
+    d_typing E (dexp_abs e) d_typingmode_chk (dtyp_arrow T1 T2)
+| d_typing_chkall : forall (L:vars) (E:denv) (e:dexp) (T1:dtyp),
+    dwf_typ E (dtyp_all T1) ->
+    ( forall X , X \notin  L  -> d_typing  ( X ~ dbind_tvar_empty  ++  E )  e  d_typingmode_chk ( open_dtyp_wrt_dtyp T1 (dtyp_var_f X) )  )  ->
+    d_typing E e d_typingmode_chk (dtyp_all T1)
+| d_typing_chksub : forall (E:denv) (e:dexp) (T1 S1:dtyp),
+    d_typing E e d_typingmode_inf S1 ->
+    d_sub E S1 T1 ->
+    d_typing E e d_typingmode_chk T1
+| d_typing_chkintersection : forall (E:denv) (e:dexp) (S1 T1:dtyp),
+    d_typing E e d_typingmode_chk S1 ->
+    d_typing E e d_typingmode_chk T1 ->
+    d_typing E e d_typingmode_chk (dtyp_intersection S1 T1)
+| d_typing_chkunion1 : forall (E:denv) (e:dexp) (S1 T1:dtyp),
+    d_typing E e d_typingmode_chk S1 ->
+    dwf_typ E T1 ->
+    d_typing E e d_typingmode_chk (dtyp_union S1 T1)
+| d_typing_chkunion2 : forall (E:denv) (e:dexp) (S1 T1:dtyp),
+    d_typing E e d_typingmode_chk T1 ->
+    dwf_typ E S1 ->
+    d_typing E e d_typingmode_chk (dtyp_union S1 T1)
+.
